acl2svn/branches/centaur/history-management.lisp
@@ -18300,11 +18300,11 @@
 
 (defun@par translate-hints1 (name-tree lst hint-type override-hints ctx wrld state)
 
-; A note on the taxonomy of hints.  A "hint setting" is a pair of the
-; form (key . val), such as (:DO-NOT-INDUCT . T) or (:USE . (lmi-lst
-; (h1...hn) ...)).  List of such pairs are called "hint settings."  A
-; pair consisting of a clause-id and some hint-settings is called a
-; "hint".  A list of such pairs is called "hints."
+; A note on the taxonomy of translated hints.  A "hint setting" is a pair of
+; the form (key . val), such as (:DO-NOT-INDUCT . T) or (:USE . (lmi-lst
+; (h1...hn) ...)).  Lists of such pairs are called "hint settings."  A pair
+; consisting of a clause-id and some hint-settings is called a "(translated)
+; hint".  A list of such pairs is called "(translated) hints."
 
 ; Thus, following the :HINTS keyword to defthm, the user types "hints" (in
 ; untranslated form).  This function takes a lst, which is supposed be some
@@ -18457,23 +18457,25 @@
   hint keywords and their values, whose source is either an explicit hint
   ~c[(goal-name :key1 val1 ... :keyn valn)] where the ~c[:keyi] are allowed to
   be custom hint keywords (which are expanded away; ~pl[custom-keyword-hints]),
-  or else is the non-~c[nil] result from evaluating a computed hint.  Then the
-  override-hints are applied to that keyword-alist as follows, one at a time,
-  in order of their occurrence in the list of override-hints (as determined by
-  the use of ~ilc[set-override-hints] and ~ilc[add-override-hints]).  The first
-  override-hint is evaluated, in the usual manner of evaluating computed hints
-  but with the variable ~c[KEYWORD-ALIST] bound to the above keyword-alist.
-  That evaluation produces a result that should also be a keyword-alist, or
-  else an error occurs.  Any custom keyword hints are then eliminated from that
-  keyword-alist.  The resulting keyword-alist must not contain the ~c[:ERROR]
-  hint keyword and must not start with the ~c[:COMPUTED-HINT-REPLACEMENT]
-  keyword; otherwise an error occurs.  With ~c[KEYWORD-ALIST] bound to this
-  result, the second override-hint is similarly evaluated.  This process
-  continues, and the keyword-alist returned by the final override-hint is the
-  one used when processing the goal at hand.  If the final result is ~c[nil],
-  then the hint is discarded and the remaining hints are considered as above,
-  regardless of whether the tentatively selected hint object came from a
-  computed hint or from an explicit hint.
+  or else is the non-~c[nil] keyword-alist produced by evaluating a computed
+  hint.  Then the override-hints are applied to that keyword-alist as follows,
+  one at a time, in order of their occurrence in the list of override-hints (as
+  determined by the use of ~ilc[set-override-hints] and
+  ~ilc[add-override-hints]).  The first override-hint is evaluated, in the
+  usual manner of evaluating computed hints but with the variable
+  ~c[KEYWORD-ALIST] bound to the above keyword-alist.  That evaluation produces
+  a result that should also be a keyword-alist, or else an error occurs.  Any
+  custom keyword hints are then eliminated from that keyword-alist.  The
+  resulting keyword-alist must not contain the ~c[:ERROR] hint keyword and must
+  not start with the ~c[:COMPUTED-HINT-REPLACEMENT] keyword; otherwise an error
+  occurs.  With ~c[KEYWORD-ALIST] bound to this result, the second
+  override-hint is similarly evaluated.  This process continues, and the
+  keyword-alist returned by the final override-hint is the one used when
+  processing the goal at hand.  Except: If that keyword-alist is ~c[nil], then
+  the next hint among the pending hints is tentatively selected and the process
+  repeats, applying each override hint to that new tentative selection.  Of
+  course we might obtain ~c[nil] again, in which case we tentatively select the
+  next pending hint; and so on.
 
   If finally no hint is selected for the current goal, then ~c[KEYWORD-ALIST]
   is bound to ~c[nil] and the override-hints are applied as described above.
@@ -19131,7 +19133,7 @@
   ~pl[hints] for an introduction to ACL2 hints, including detailed
   ~il[documentation] for specific hint types.
 
-  The remainder of this topic serves as a references in case one needs a deeper
+  The remainder of this topic serves as a reference in case one needs a deeper
   understanding of the workings of ACL2's handling of hints.  Also, for
   examples of the sophisticated use of hints, primarily for experts, see
   distributed book ~c[books/hints/basic-tests.lisp].
@@ -19169,7 +19171,7 @@
   settling down has occurred and modify their heuristics accordingly.)  For
   example, if ~c[\"Goal\"] simplifies to ~c[\"Subgoal 2\"] (among others), and
   ~c[\"Subgoal 2\"] simplifies to ~c[\"Subgoal 2.3\"] (among others), which in
-  turn is not further simplified, then the the ``settled-down'' process hits on
+  turn is not further simplified, then the ``settled-down'' process hits on
   ~c[\"Subgoal 2.3\"] but not on any of its children, their children, and so
   on.
 
@@ -19218,22 +19220,23 @@
   The list of hint settings associates hint keywords with values.  It is passed
   from the current goal to its children (and hence the children's children, and
   so on), though modified by hints selected from pending hints, as described
-  below.  This list is consulted when a goal is pushed for later proof by
-  induction, at which time the hint settings are stored so that when the
-  induction proof begins, it begins with those hint settings.  Note that the
-  list of hint settings is not re-applied to descendents of a goal; a hint is
-  applied only when it is selected.  For example, if the hint selected for
-  ~c[\"Subgoal 3\"] includes ~c[:in-theory (enable foo)], then the hint
-  settings are correspondingly updated when processing ~c[\"Subgoal 3\"], and
-  they persist at subgoals such as ~c[\"Subgoal 3.2\"] and
-  ~c[\"Subgoal 3.2.1\"] (unless overriden by hints on those goals); but the
+  below.  This list is maintained so that when a goal is pushed for proof by
+  induction, the hint settings are applied at the start of the proof by
+  induction.  Note that the list of hint settings is not re-applied to
+  descendents of a goal in the current waterfall; a hint is applied only when
+  it is selected (and also perhaps later as just described, through the stored
+  hint settings at the start of a proof by induction).  For example, if the
+  hint selected for ~c[\"Subgoal 3\"] includes ~c[:in-theory (enable foo)],
+  then the hint settings are correspondingly updated when processing
+  ~c[\"Subgoal 3\"], and they persist at subgoals such as ~c[\"Subgoal 3.2\"]
+  and ~c[\"Subgoal 3.2.1\"] (unless overriden by hints on those goals); but the
   theory specifying ~c[foo] is not re-installed at every such subgoal.
 
-  When a hint is selected, the list of hint-settings is updated so that for
+  When a hint is selected, the list of hint settings is updated so that for
   each keyword ~c[:kwd] and associated value ~c[val] from the hint, ~c[:kwd] is
-  associated with ~c[val] in the hint-settings, discarding any previous
-  association of ~c[:kwd] with a value in the hint-settings.  Except, certain
-  ``top-level'' hints are never saved in the hint-settings: ~c[:use],
+  associated with ~c[val] in the hint settings, discarding any previous
+  association of ~c[:kwd] with a value in the hint settings.  Except, certain
+  ``top-level'' hints are never saved in the hint settings: ~c[:use],
   ~c[:cases], ~c[:by], ~c[:bdd], ~c[:or], and ~c[:clause-processor].
 
   For example, suppose that we specify the following hints, with no default
@@ -19263,16 +19266,16 @@
   ~c[:in-theory] association is removed from the hint settings and the global
   theory is re-installed.  However, the list of pending hints remains empty.
 
-  It remains to describe how hints are chosen for a goal.  When a goal is first
-  considered (hence at the top of the waterfall), the list of pending hints is
-  scanned, in order, until one of the hints is suitable for the goal.  An
-  explicit hint ~c[(goal-name :kwd1 val1 ... :kwdn valn)] is suitable if
+  It remains to describe how a hint is selected for a goal.  When a goal is
+  first considered (hence at the top of the waterfall), the list of pending
+  hints is scanned, in order, until one of the hints is suitable for the goal.
+  An explicit hint ~c[(goal-name :kwd1 val1 ... :kwdn valn)] is suitable if
   ~c[goal-name] is the name of the current goal and there is at least one
-  keyword.  A computed hint is suitable if it evaluates to a non-~c[nil]
-  value.  As indicated earlier in this documentation topic, an exception occurs
-  when a computed hint is selected after simplification fails (the
+  keyword.  A computed hint is suitable if it evaluates to a non-~c[nil] value.
+  As indicated earlier in this documentation topic, an exception occurs when a
+  computed hint is selected after simplification fails (the
   ``~c[stable-under-simplificationp]'' case): in that case, the goal returns to
-  the top of the waterfall with that hint is the selected hint, and no
+  the top of the waterfall with that hint as the selected hint, and no
   additional search for a hint to select is made at that time.
 
   The following slightly tricky example illustrates handling of hints.
@@ -19298,17 +19301,17 @@
   ~ev[]
 
   The warning above is printed because ~c[\"Goal\"] is associated with two
-  hints: one given by the ~ilc[set-default-hints] call and one supplied by the
-  ~c[:]~ilc[hints] keyword of the ~ilc[thm] form.  The ~c[:in-theory] hint is
-  selected because user-supplied hints are ahead of default hints in the list
-  of hints to consider; we then get the first ``Note'' above.  The goal
+  pending hints: one given by the ~ilc[set-default-hints] call and one supplied
+  by the ~c[:]~ilc[hints] keyword of the ~ilc[thm] form.  The ~c[:in-theory]
+  hint is selected because user-supplied hints are ahead of default hints in
+  the list of pending hints; we then get the first ``Note'' above.  The goal
   progresses through the waterfall without any proof process applying to the
   goal; in particular, it cannot be further simplified.  After the
   simplification process, a ``settled-down'' process applies, as discussed
-  above, immediately causing another trip through the waterfall.  At that point
-  the ~c[:in-theory] hint had previously been removed when it was applied,
-  leaving the default (~c[:do-not]) hint as the only applicable hint.  That
-  hint is indeed applied, resulting in the second ``Note'' above.
+  above, immediately causing another trip through the waterfall.  Since the
+  ~c[:in-theory] hint was earlier removed from the list of pending hints when
+  it was applied, the default (~c[:do-not]) hint is now the only pending hint.
+  That hint is applied, resulting in the second ``Note'' above.
 
   Again, more examples may be found in the distributed book
   ~c[books/hints/basic-tests.lisp].  A particularly tricky but informative
@@ -20042,16 +20045,19 @@
   returns ~c[nil], then the ~c[:backtrack] hint has no effect, and the goal is
   replaced by the list of goals (the value of ~c[CLAUSE-LIST] described above),
   as usual.  Otherwise, the clause processor is deemed to have failed, and the
-  goal clause is tried again after applying the hint returned by the above
-  evaluation.  That hint will normally be an alternating list of hint keywords
-  and their values, but if it is a custom keyword hint
-  (~pl[custom-keyword-hints]), then it will be handled in the usual manner but
-  with the first three variables above bound to the symbol ~c[:OMITTED].  Of
-  course, if the new hint includes a value for ~c[:BACKTRACK] then this process
-  can loop; care should be taken to keep that from happening.
+  goal clause is tried again starting at the top of the waterfall after
+  selecting the hint returned by the above evaluation.  That hint will normally
+  be an alternating list of hint keywords and their values, but if it is a
+  custom keyword hint (~pl[custom-keyword-hints]), then it will be handled in
+  the usual manner but with the first three variables above bound to the symbol
+  ~c[:OMITTED].  Of course, if the new hint includes a value for ~c[:BACKTRACK]
+  then this process can loop; care should be taken to keep that from happening.
 
-  A final note about ~c[:BACKTRACK] hints: ~il[override-hints] (if any) are
-  applied in their processing.  ~l[override-hints].~/")
+  A final note about ~c[:BACKTRACK] hints: since these are a form of computed
+  hints, ~il[override-hints] (if any) are applied to their evaluation result
+  just as with any computed hint.  That is, the backtrack hint is successively
+  modified with each override-hint, to produce a final hint that is actually
+  used (or, ignored if that final hint is ~c[nil]).  ~l[override-hints].~/")
 
 (deflabel clause-identifier
   :doc
