acl2svn/branches/centaur/translate.lisp
@@ -371,25 +371,6 @@
          (remove-keyword word (cddr l)))
         (t (list* (car l) (cadr l) (remove-keyword word (cddr l))))))
 
-(defun ignored-attachment-msg (prefix ignored-attachment)
-  (cond (ignored-attachment (msg "~@0Note that because of logical ~
-                                  considerations, attachments (including ~x1) ~
-                                  must not be called in this context."
-                                 prefix ignored-attachment))
-        (t "")))
-
-(defun ev-fncall-null-body-er (ignored-attachment fn latches)
-  (mv t
-      (msg "ACL2 cannot evaluate the undefined function ~x0.~@1"
-           fn
-           (ignored-attachment-msg "  " ignored-attachment))
-      latches))
-
-(defconst *safe-mode-guard-er-addendum*
-  "  The guard is being checked because this function is a primitive and a ~
-   \"safe\" mode is being used for defconst, defpkg, macroexpansion, or ~
-   another operation where safe mode is required.")
-
 (defun error-trace-suggestion (two-leading-spaces)
 
 ; Warning: Do not eliminate the message about print-gv without first reading
@@ -400,6 +381,65 @@
        (if two-leading-spaces
            "  "
          "")))
+
+(defun ignored-attachment-msg (ignored-attachment)
+  (cond (ignored-attachment (msg "~|~%Note that because of logical ~
+                                  considerations, attachments (including ~x0) ~
+                                  must not be called in this context."
+                                 ignored-attachment))
+        (t "")))
+
+(defun ev-fncall-null-body-er-msg (ignored-attachment fn args)
+  (msg "ACL2 cannot ev the call of undefined function ~x0 on argument ~
+        list:~|~%~x1~@2~|~%~@3"
+       fn
+       args
+       (ignored-attachment-msg ignored-attachment)
+       (error-trace-suggestion nil)))
+
+(defun ev-fncall-null-body-er (ignored-attachment fn args latches)
+  (mv t
+      (ev-fncall-null-body-er-msg ignored-attachment fn args)
+      latches))
+
+(defun ev-fncall-creator-er-msg (fn)
+  (msg
+   "An attempt has been made to call the stobj creator function ~x0.  This ~
+    error is being reported even though guard-checking may have been turned ~
+    off, because ACL2 does not support non-compliant live stobj manipulation. ~
+    ~ If you did not explicitly call ~x0 then this error is probably due to ~
+    an attempt to evaluate a with-local-stobj form directly in the top-level ~
+    loop.  Such forms are only allowed in the bodies of functions and in ~
+    theorems.  Also see :DOC with-local-stobj.~@1"
+   fn
+   (error-trace-suggestion t)))
+
+(defun unknown-pkg-error-msg (fn pkg-name)
+  (msg
+   "The call ~x0 is illegal because the argument is not the name of a ~
+      package currently known to ACL2."
+   (list fn pkg-name)))
+
+(defun illegal-msg ()
+  (msg "Evaluation aborted.~@0"
+       (error-trace-suggestion t)))
+
+(defun program-only-er-msg (fn args safe-mode)
+  (msg
+   "The call ~x0 is an illegal call of a function that has been marked as ~
+    ``program-only,'' and hence has special raw Lisp code.  This call is ~
+    illegal because program-only functions are only allowed to invoke their ~
+    raw Lisp code, but in this case there was an attempt to invoke executable ~
+    counterpart code ~#1~[because of guard-checking (see :DOC ~
+    guard-evaluation-table)~/because it is being called under a ``safe mode'' ~
+    that is used, for example, during macroexpansion~]."
+   (cons fn args)
+   (if safe-mode 1 0)))
+
+(defconst *safe-mode-guard-er-addendum*
+  "  The guard is being checked because this function is a primitive and a ~
+   \"safe\" mode is being used for defconst, defpkg, macroexpansion, or ~
+   another operation where safe mode is required.")
 
 (defun find-first-non-nil (lst)
   (cond ((endp lst) nil)
@@ -1471,54 +1511,80 @@
          (mv nil x latches))
         #+:non-standard-analysis
         (I-LARGE-INTEGER ; We could omit this case, allowing a fall-through.
-         (ev-fncall-null-body-er nil fn latches))
+         (ev-fncall-null-body-er nil fn nil latches)) 
         (otherwise
-         (let ((alist (pairlis$ (formals fn w) args))
-               (body (body fn nil w))
-               (attachment (and aok
-                                (cdr (assoc-eq fn (all-attachments w))))))
-           (mv-let
-            (er val latches)
-            (ev-rec (if guard-checking-off
-                        ''t
-                      (guard fn nil w))
-                    alist
-                    w (decrement-big-n big-n) (eq extra t) guard-checking-off
-                    latches
-                    hard-error-returns-nilp
-                    aok)
-            (cond
-             (er (mv er val latches))
-             ((null val)
-              (ev-fncall-guard-er fn args w latches extra))
-             (attachment
-              (ev-fncall-rec-logical attachment args w
-                                     (decrement-big-n big-n)
-                                     safe-mode gc-off latches
-                                     hard-error-returns-nilp aok))
-             ((null body)
-              (ev-fncall-null-body-er
-               (and (not aok) attachment)
-               fn latches))
-             (t
-              (mv-let
-               (er val latches)
-               (ev-rec body alist
-                       w (decrement-big-n big-n) (eq extra t)
-                       guard-checking-off
-                       latches
-                       hard-error-returns-nilp
-                       aok)
-               (cond
-                (er (mv er val latches))
-                ((eq fn 'return-last) ; avoid taking stobjs-out of return-last
-                 (mv nil val latches))
-                (t (mv nil
-                       val
-                       (latch-stobjs
-                        (stobjs-out fn w)
-                        val
-                        latches)))))))))))))))
+         (cond
+          ((and (null args)
+                (car (stobjs-out fn w)))
+           (mv t
+               (ev-fncall-creator-er-msg fn)
+               latches))
+          (t
+           (let ((alist (pairlis$ (formals fn w) args))
+                 (body (body fn nil w))
+                 (attachment (and aok
+                                  (cdr (assoc-eq fn (all-attachments w))))))
+             (mv-let
+              (er val latches)
+              (ev-rec (if guard-checking-off
+                          ''t
+                        (guard fn nil w))
+                      alist
+                      w (decrement-big-n big-n) (eq extra t) guard-checking-off
+                      latches
+                      hard-error-returns-nilp
+                      aok)
+              (cond
+               (er (mv er val latches))
+               ((null val)
+                (ev-fncall-guard-er fn args w latches extra))
+               ((and (eq fn 'hard-error)
+                     (not hard-error-returns-nilp))
+
+; Before we added this case, the following returned nil even though the result
+; was t if we replaced ev-fncall-rec-logical by ev-fncall-rec.  That wasn't
+; quite a soundness bug, event though the latter is defined to be the former,
+; because ev-fncall-rec is untouchable; nevertheless the discrepancy was
+; troubling.
+ 
+;   (mv-let (erp val ign)
+;           (ev-fncall-rec-logical 'hard-error '(top "ouch" nil) (w state)
+;                                  100000 nil nil nil nil t)
+;           (declare (ignore ign val))
+;           erp)
+
+         
+                (mv t (illegal-msg) latches))
+               ((member-eq fn '(pkg-witness pkg-imports))
+                (mv t (unknown-pkg-error-msg fn (car args)) latches))
+               (attachment
+                (ev-fncall-rec-logical attachment args w
+                                       (decrement-big-n big-n)
+                                       safe-mode gc-off latches
+                                       hard-error-returns-nilp aok))
+               ((null body)
+                (ev-fncall-null-body-er
+                 (and (not aok) attachment)
+                 fn args latches))
+               (t
+                (mv-let
+                 (er val latches)
+                 (ev-rec body alist
+                         w (decrement-big-n big-n) (eq extra t)
+                         guard-checking-off
+                         latches
+                         hard-error-returns-nilp
+                         aok)
+                 (cond
+                  (er (mv er val latches))
+                  ((eq fn 'return-last) ; avoid stobjs-out for return-last
+                   (mv nil val latches))
+                  (t (mv nil
+                         val
+                         (latch-stobjs
+                          (stobjs-out fn w)
+                          val
+                          latches)))))))))))))))))
 
 (defun ev-fncall-rec (fn args w big-n safe-mode gc-off latches
                          hard-error-returns-nilp aok)
@@ -2232,18 +2298,13 @@
       latches))
 
 (defun ev-fncall-msg (val wrld)
+
+; Warning: Keep this in sync with ev-fncall-rec-logical.
+
   (cond
    ((and (consp val)
          (eq (car val) 'ev-fncall-null-body-er))
-
-; We get here if val is of the form (ev-fncall-null-body-er fn).
-
-    (msg "ACL2 cannot ev the call of undefined function ~x0 on argument ~
-          list:~|~%~x1~@2~|~%~@3"
-         (caddr val)
-         (cdddr val)
-         (ignored-attachment-msg "~|~%" (cadr val))
-         (error-trace-suggestion nil)))
+    (ev-fncall-null-body-er-msg (cadr val) (caddr val) (cdddr val)))
    ((and (consp val)
          (eq (car val) 'ev-fncall-guard-er))
 
@@ -2259,44 +2320,25 @@
 
 ; This is similar to the preceding case, except that there are no stobjs-in.
 
-    (msg
-     "An attempt has been made to call the stobj creator function ~x0.  This ~
-      error is being reported even though guard-checking may have been turned ~
-      off, because ACL2 does not support non-compliant live stobj ~
-      manipulation.  If you did not explicitly call ~x0 then this error is ~
-      probably due to an attempt to evaluate a with-local-stobj form directly ~
-      in the top-level loop.  Such forms are only allowed in the bodies of ~
-      functions and in theorems.  Also see :DOC with-local-stobj.~@1"
-     (cadr val)
-     (error-trace-suggestion t)))
+    (ev-fncall-creator-er-msg
+     (cadr val)))
    ((and (consp val)
-         (eq (car val) 'pkg-witness-er))
-    (msg
-     "The call ~x0 is illegal because the second argument is not the name of a ~
-      package currently known to ACL2."
-     (list 'pkg-witness (cadr val))))
-   ((and (consp val)
-         (eq (car val) 'pkg-imports-er))
-    (msg
-     "The call ~x0 is illegal because the argument is not the name of a ~
-      package currently known to ACL2."
-     (list 'pkg-imports (cadr val))))
-   ((and (consp val)
-         (eq (car val) 'program-only-er))
-    (msg
-     "The call ~x0 is an illegal call of a function that has been marked as ~
-      ``program-only,'' and hence has special raw Lisp code.  This call is ~
-      illegal because program-only functions are only allowed to invoke their ~
-      raw Lisp code, but in this case there was an attempt to invoke ~
-      executable counterpart code ~#2~[because of guard-checking (see :DOC ~
-      guard-evaluation-table)~/because it is being called under a ``safe ~
-      mode'' that is used, for example, during macroexpansion~]."
-     (cons (cadr val) (caddr val))
-     (cadr val)
-     (if (cadr (cddddr val)) 1 0)))
+         (member-eq (car val) '(pkg-witness-er pkg-imports-er)))
+    (unknown-pkg-error-msg (car val) (cadr val)))
+
+; At one time we had the following case:
+
+;  ((and (consp val)
+;        (eq (car val) 'program-only-er))
+
+; In this case we (essentially) returned (program-only-er-msg (cadr val) (caddr
+; val) (cadr (cddddr val))).  But we get here by catching a throw of val, which
+; no longer is of the form (program-only-er ...); see the comment about the
+; call of oneify-fail-form on 'program-only-er (and other arguments) in
+; oneify-cltl-code.
+
    ((eq val 'illegal)
-    (msg "Evaluation aborted.~@0"
-         (error-trace-suggestion t)))
+    (illegal-msg))
    (t (er hard 'raw-ev-fncall
           "An unrecognized value, ~x0, was thrown to 'raw-ev-fncall.~@1"
           val
@@ -2489,7 +2531,9 @@
                          (let* ((key (unquote (fargn term 1)))
                                 (fn (and (symbolp key)
                                          key
-                                         (return-last-lookup key wrld))))
+                                         (let ((tmp (return-last-lookup key
+                                                                        wrld)))
+                                           (if (consp tmp) (car tmp) tmp)))))
                            (and fn
                                 (cons fn
                                       (untranslate1-lst (cdr (fargs term)) nil
@@ -4637,6 +4681,27 @@
     brr-gstack
     brr-alist))
 
+(defun unknown-binding-msg-er (x ctx stobjs-bound str1 str2 str3)
+  (mv-let
+   (erp msg bindings)
+   (let ((bindings nil)) ; don't-care
+     (trans-er+
+      x ctx
+      "~@0"
+      (msg "The single-threaded object~#0~[ ~&0 has~/s ~&0 have~] been bound ~
+            in ~@1.  It is a requirement that ~#0~[this object~/these ~
+            objects~] be among the outputs of ~@2.  But, at the time at which ~
+            we process ~@2, we are unable to determine what the outputs are ~
+            and so cannot allow it.  This situation can arise when the output ~
+            of ~@2 is a recursive call of the function being admitted and no ~
+            other IF branch of the body of the function (or in the case of ~
+            mutual recursion, the body of any other function in the clique) ~
+            tells us the output signature of the function.  Perhaps a ~
+            recursion's base case is missing."
+           stobjs-bound str1 str2 str3)))
+   (declare (ignore bindings))
+   (mv erp msg :UNKNOWN-BINDINGS)))
+
 (mutual-recursion
 
 (defun translate11-flet-alist (form fives stobjs-out bindings known-stobjs
@@ -4711,11 +4776,7 @@
                                               bindings))
                             known-stobjs
                             flet-alist form ctx wrld state-vars)))
-       (let ((stobjs-bound
-              (collect-non-x nil (compute-stobj-flags bound-vars
-                                                      known-stobjs
-                                                      wrld)))
-             (used-vars (union-eq (all-vars tbody)
+       (let ((used-vars (union-eq (all-vars tbody)
                                   (all-vars1-lst tdcls nil)))
              (ignore-vars (ignore-vars edcls))
              (ignorable-vars (ignorable-vars edcls))
@@ -4723,17 +4784,28 @@
          (cond
 
 ; We skip the following case, where stobjs-out is not yet bound to a consp and
-; some formal is a stobj, in favor of the next, which removes the stobj
+; some formal is a stobj, in favor of the next, which removes the stobjs-bound
 ; criterion.  But we leave this case here as a comment in case we ultimately
-; find a way to eliminate the more sweeping case after it.
+; find a way to eliminate the more sweeping case after it.  Note: 
+; unknown-binding-msg has been replaced by unknown-binding-msg-er, so a bit of
+; rework will be needed if this case is to be reinstalled.  Also note that we
+; will need to bind stobjs-bound to
 
 ;         ((and (not (eq stobjs-out t))
-;               stobjs-bound
+;               (collect-non-x ; stobjs-bound
+;                nil
+;                (compute-stobj-flags bound-vars
+;                                     known-stobjs
+;                                     wrld))
 ;               (not (consp stobjs-out)))
 ;          (trans-er ctx
 ;                    "~@0"
 ;                    (unknown-binding-msg
-;                     stobjs-bound
+;                     (collect-non-x ; stobjs-bound
+;                      nil
+;                      (compute-stobj-flags bound-vars
+;                                           known-stobjs
+;                                           wrld))
 ;                     (msg "the formals of an FLET binding for function ~x0"
 ;                          name)
 ;                     "the body of this FLET binding"
@@ -4745,6 +4817,10 @@
 ; Warning: Before changing this case, see the comment above about the
 ; commented-out preceding case.
 
+; We might be able to fix this case by using the :UNKNOWN-BINDINGS trick
+; employed by unknown-binding-msg-er; see that function and search for
+; :UNKNOWN-BINDINGS, to see how that works.
+
            (trans-er+ form ctx
                       "We are unable to determine the output signature for an ~
                        FLET-binding of ~x0.  You may be able to remedy the ~
@@ -4755,23 +4831,6 @@
                        ACL2 should be able to complete this translation, ~
                        please send such an example to the ACL2 implementors."
                      name))
-          ((and (not (eq stobjs-out t))
-                stobjs-bound
-                (not (subsetp-eq stobjs-bound
-                                 (collect-non-x nil stobjs-out))))
-           (let ((stobjs-returned (collect-non-x nil stobjs-out)))
-             (trans-er+ form ctx
-                        "The single-threaded object~#0~[ ~&0 is a formal~/s ~
-                         ~&0 are formals~] of an FLET-binding of ~x3.  It is ~
-                         a requirement that ~#0~[this object~/these objects~] ~
-                         be among the outputs of the body of that binding, ~
-                         but ~#0~[it is~/they are~] not.  That body returns ~
-                         ~#1~[no single-threaded objects~/the single-threaded ~
-                         object ~&2~/the single-threaded objects ~&2~]."
-                       (set-difference-eq stobjs-bound stobjs-returned)
-                       (zero-one-or-more stobjs-returned)
-                       stobjs-returned
-                       name)))
           ((intersectp-eq used-vars ignore-vars)
            (trans-er+ form ctx
                       "Contrary to the declaration that ~#0~[it is~/they ~
@@ -5028,10 +5087,8 @@
                          local-stobj))
              ((and stobjs-bound
                    (not (consp stobjs-out)))
-              (trans-er+ x ctx
-                         "~@0"
-                         (unknown-binding-msg
-                          stobjs-bound "an MV-LET" "the MV-LET" "the MV-LET")))
+              (unknown-binding-msg-er x ctx stobjs-bound
+                                      "an MV-LET" "the MV-LET" "the MV-LET"))
              ((and stobjs-bound
                    (not (subsetp stobjs-bound
                                  (collect-non-x nil stobjs-out))))
@@ -5338,7 +5395,8 @@
 ;                  of its body, as we translate.  We also enforce prohibitions
 ;                  against the use of DEFUN, IN-PACKAGE, etc inside bodies.
 ; :stobjs-out    - like a function name, except we know we are NOT in a defun
-;                  body and allow DEFUN, IN-PACKAGE, etc.
+;                  body and allow DEFUN, IN-PACKAGE, etc., but restrict certain
+;                  calls of return-last.
 
 ; See the essay on STOBJS-IN and STOBJS-OUT, above.
 
@@ -5618,7 +5676,7 @@
                       #+:non-standard-analysis defthm-std
                       #+:non-standard-analysis defun-std
                       add-custom-keyword-hint
-                      add-include-book-dir
+                      add-include-book-dir ; definition explains inclusion here
                       add-match-free-override
                       certify-book
                       comp
@@ -5632,7 +5690,7 @@
                       deftheory
                       defthm
                       defuns
-                      delete-include-book-dir
+                      delete-include-book-dir ; definition explains inclusion
                       encapsulate
                       in-arithmetic-theory
                       in-theory
@@ -5971,10 +6029,8 @@
                  ((and (not (eq stobjs-out t))
                        stobjs-bound
                        (not (consp stobjs-out)))
-                  (trans-er+ x ctx
-                             "~@0"
-                             (unknown-binding-msg
-                              stobjs-bound "a LET" "the LET" "the LET")))
+                  (unknown-binding-msg-er x ctx stobjs-bound
+                                          "a LET" "the LET" "the LET"))
                  ((and (not (eq stobjs-out t))
                        stobjs-bound
                        (not (subsetp-eq stobjs-bound
@@ -6091,30 +6147,56 @@
                        on untouchable-fns."
                       (car x)))
           ((eq (car x) 'if)
-           (cond ((stobjp (cadr x) known-stobjs wrld)
-                  (trans-er+ x ctx
-                             "It is illegal to test on a single-threaded ~
-                              object such as ~x0."
-                             (cadr x)))
+           (cond
+            ((stobjp (cadr x) known-stobjs wrld)
+             (trans-er+ x ctx
+                        "It is illegal to test on a single-threaded object ~
+                         such as ~x0."
+                        (cadr x)))
 
 ; Because (cadr x) has not yet been translated, we do not really know it is not
 ; a stobj!  It could be a macro call that expands to a stobj.'  The error
 ; message above is just to be helpful.  An accurate check is made below.
 
-                 (t (trans-er-let*
-                     ((arg1 (translate11 (cadr x)
-                                         (if (eq stobjs-out t)
-                                             t
-                                           '(nil))
-                                         bindings known-stobjs
-                                         flet-alist x ctx wrld state-vars))
-                      (arg2 (translate11 (caddr x)
-                                         stobjs-out bindings known-stobjs
-                                         flet-alist x ctx wrld state-vars))
-                      (arg3 (translate11 (cadddr x)
-                                         stobjs-out bindings known-stobjs
-                                         flet-alist x ctx wrld state-vars)))
-                     (trans-value (fcons-term* 'if arg1 arg2 arg3))))))
+            (t
+             (trans-er-let*
+              ((arg1 (translate11 (cadr x)
+                                  (if (eq stobjs-out t)
+                                      t
+                                    '(nil))
+                                  bindings known-stobjs
+                                  flet-alist x ctx wrld state-vars)))
+              (mv-let
+               (erp2 arg2 bindings2)
+               (trans-er-let*
+                ((arg2 (translate11 (caddr x)
+                                    stobjs-out bindings known-stobjs
+                                    flet-alist x ctx wrld state-vars)))
+                (trans-value arg2))
+               (cond
+                (erp2
+                 (cond
+                  ((eq bindings2 :UNKNOWN-BINDINGS)
+                   (mv-let
+                    (erp3 arg3 bindings)
+                    (translate11 (cadddr x)
+                                 stobjs-out bindings known-stobjs
+                                 flet-alist x ctx wrld state-vars)
+                    (cond
+                     (erp3 (mv erp2 arg2 bindings2))
+                     (t (trans-er-let*
+                         ((arg2 (translate11 (caddr x)
+                                             stobjs-out bindings known-stobjs
+                                             flet-alist x ctx wrld state-vars)))
+                         (trans-value (fcons-term* 'if arg1 arg2 arg3)))))))
+                  (t (mv erp2 arg2 bindings2))))
+                (t
+                 (let ((bindings bindings2))
+                   (trans-er-let*
+                    ((arg3 (translate11 (cadddr x)
+                                        stobjs-out bindings known-stobjs
+                                        flet-alist x ctx wrld state-vars)))
+                    (trans-value (fcons-term* 'if arg1 arg2 arg3)))))))))))
           ((eq (car x) 'synp)
 
 ; Synp is a bit odd.  We store the quotation of the term to be evaluated in the
@@ -6229,6 +6311,16 @@
             ((args (translate11-lst (cdr x) t bindings known-stobjs
                                     nil flet-alist x ctx wrld state-vars)))
             (trans-value (fcons-term (car x) args))))
+          ((eq (getprop (car x) 'non-executablep nil 'current-acl2-world
+                        wrld)
+               t)
+           (let ((computed-stobjs-out (compute-stobj-flags (cdr x)
+                                                           known-stobjs
+                                                           wrld)))
+             (trans-er-let*
+              ((args (translate11-lst (cdr x) computed-stobjs-out bindings known-stobjs
+                                      nil flet-alist x ctx wrld state-vars)))
+              (trans-value (fcons-term (car x) args)))))
           ((eq (car x) 'return-last) ; and stobjs-out is not t
            (let* ((arg1 (nth 1 x))
                   (key (and (consp arg1)
@@ -6308,7 +6400,11 @@
                                   (t (msg "~x0 is a macro, not a function ~
                                            symbol"
                                           fn))))))
-               ((and keyp (not (return-last-lookup key wrld)))
+               ((and keyp
+                     (let ((val (return-last-lookup key wrld)))
+                       (or (null val)
+                           (and (consp val) ; see chk-return-last-entry
+                                (eq stobjs-out :stobjs-out)))))
 
 ; In an early implementation of return-last, we insisted that keyp be true.  But
 ; when we attempted to update the "GL" work of Sol Swords to use return-last,
@@ -6318,12 +6414,25 @@
 ; want to write meta-level functions that cons up return-last terms without a
 ; quoted first argument; and since it is easy to support that, we do so.
 
-                (trans-er ctx
-                          "The symbol ~x0 is specified in the first argument ~
-                           of the form ~x1.  But ~x0 is not associated in the ~
-                           table ~x2 with a non-nil symbol.  See :DOC ~
-                           return-last."
-                          key x 'return-last-table))
+                (cond
+                 ((null (return-last-lookup key wrld))
+                  (trans-er ctx
+                            "The symbol ~x0 is specified in the first ~
+                             argument of the form ~x1.  But ~x0 is not ~
+                             associated in the table ~x2 with a non-nil ~
+                             value.  See :DOC return-last."
+                            key x 'return-last-table))
+                 (t
+                  (trans-er ctx
+                            "Illegal call, ~x0: the association of ~x1 with ~
+                             the symbol ~x2 has been restricted to avoid ~
+                             top-level evaluation of such calls of ~x3.  See ~
+                             :DOC return-last.  Also consider placing the ~
+                             offending call inside a call of ~x4; see :DOC ~
+                             ~x4."
+                            x key
+                            (car (return-last-lookup key wrld))
+                            'return-last 'top-level))))
                (t
                 (mv-let
                  (erp targ2 targ2-bindings)
@@ -6467,7 +6576,7 @@
                             msg flet-alist cform ctx wrld state-vars)
 
 ; WARNING: This function's treatment of stobjs-out is unusual:
-; (1) stobjs-out must be either t, nil, or list of stobjs flags.
+; (1) stobjs-out must be either t, nil, or list of stobj flags.
 ;     It CANNOT be a function name (``an unknown'').
 ; (2) If stobjs-out is nil, it is treated as though it were a list of
 ;     nils as long as lst.
@@ -6587,9 +6696,7 @@
 ; function symbol except that it tells us we are NOT processing a definition
 ; body.  As is noted below, if the initial stobjs-out is :stobjs-out, bindings
 ; MUST be '((:stobjs-out . :stobjs-out)) and we use (eq (caar bindings)
-; :stobjs-out) to determine that we are not in a definition.  [Note: as this
-; function recurs, bindings may grow because we add new bindings with cons; but
-; in the case of :stobjs-out it will always contain just that one key.]
+; :stobjs-out) to determine that we are not in a definition.
 
 ; CAUTION: If you call this function with stobjs-out being a symbol, say fn,
 ; make sure that
@@ -6614,7 +6721,28 @@
 ; bindings has been modified to bind every fn (ultimately) to a proper stobjs
 ; out setting.  Use translate-deref to recover the bindings.
 
-  (translate11 x stobjs-out bindings known-stobjs nil x ctx w state-vars))
+  (trans-er-let*
+   ((result
+     (translate11 x stobjs-out bindings known-stobjs nil x ctx w state-vars)))
+   (cond ((and bindings
+               (null (cdr bindings))
+               (symbolp (caar bindings))
+               (eq (caar bindings) (cdar bindings)))
+
+; This case can happen because x is the call of a non-executable function.  We
+; return a proper stobjs-out value, for example as passed by trans-eval to
+; ev-for-trans-eval.  This treatment is necessary for the following example, to
+; avoid being unable to determine the output signature of g.
+
+; (defun-nx f (x) x)
+; (defun g (x) (f x))
+
+; This treatment is consistent with our use of stobjs-out = (nil) for
+; non-executable functions.
+
+          (trans-value result
+                       (translate-bind (caar bindings) '(nil) bindings)))
+         (t (trans-value result)))))
 
 (defun@par translate1 (x stobjs-out bindings known-stobjs ctx w state)
   (cmp-and-value-to-error-quadruple@par
